platform/XmlOutput.v
@@ -3,19 +3,70 @@ Require Import AutoSep Wrap StringOps XmlLex SinglyLinkedList Malloc.
 Set Implicit Arguments.
 
 
-(** * Compiling patterns into Bedrock chunks *)
+(** * A language for generating XML code *)
+
+Inductive xml :=
+| Cdata (data : string)
+| Tag (tag : string) (inner : list xml).
+
+Section ForallR.
+  Variable A : Type.
+  Variable P : A -> Prop.
+
+  Fixpoint ForallR (ls : list A) : Prop :=
+    match ls with
+      | nil => True
+      | x :: ls' => P x /\ ForallR ls'
+    end.
+
+  Theorem Forall_ForallR : forall ls, List.Forall P ls -> ForallR ls.
+    induction 1; simpl; intuition.
+  Qed.
+
+  Theorem ForallR_Forall : forall ls, ForallR ls -> List.Forall P ls.
+    induction ls; simpl; intuition.
+  Qed.
+End ForallR.
+
+Fixpoint wf (xm : xml) : Prop :=
+  match xm with
+    | Cdata data => goodSize (String.length data)
+    | Tag tag inner => goodSize (String.length tag + 3) /\ ForallR wf inner
+  end.
+
+Section xml_ind'.
+  Variable P : xml -> Prop.
+
+  Hypothesis H_Cdata : forall data, P (Cdata data).
+
+  Hypothesis H_Tag : forall tag inner, List.Forall P inner -> P (Tag tag inner).
+
+  Fixpoint xml_ind' (xm : xml) : P xm :=
+    match xm with
+      | Cdata data => H_Cdata data
+      | Tag tag inner => H_Tag tag ((fix xmls_ind (xms : list xml) : List.Forall P xms :=
+        match xms with
+          | nil => Forall_nil _
+          | xm :: xms' => Forall_cons _ (xml_ind' xm) (xmls_ind xms')
+        end) inner)
+    end.
+End xml_ind'.
+
+Opaque xml_ind'.
+
+
+(** * Compiling XML snippets into Bedrock chunks *)
 
 Section Out.
-  Variables start len : string.
-
-  Variable inv : vals -> HProp.
+  Variable A : Type.
+  Variables invPre invPost : A -> vals -> HProp.
 
   (* Precondition and postcondition of generation *)
   Definition invar :=
-    Al bs,
-    PRE[V] array8 bs (V "buf") * [| length bs = wordToNat (V "len") |]
-      * [| wordToNat (V start) + wordToNat (V len) <= wordToNat (V "len") |]%nat * inv V
-    POST[_] array8 bs (V "buf") * mallocHeap 0.
+    Al a : A, Al bs,
+    PRE[V] array8 bs (V "obuf") * [| length bs = wordToNat (V "olen") |]
+      * [| V "opos" <= V "olen" |] * invPre a V
+    POST[_] Ex bs', array8 bs' (V "obuf") * [| length bs' = length bs |] * invPost a V.
 
   (* Alternate sequencing operator, which generates twistier code but simpler postconditions and VCs *)
   Definition SimpleSeq (ch1 ch2 : chunk) : chunk := fun ns res =>
@@ -23,31 +74,45 @@ Section Out.
 
   Infix ";;" := SimpleSeq : SP_scope.
 
-  Notation "l ~~ im ~~> s" := (LabelMap.find l%SP im = Some (Precondition s None)) (at level 0).
+  Section OutList.
+    Variable Out' : xml -> chunk.
 
-  Notation OutVcs := (fun im ns res =>
-    (~In "rp" ns) :: In "buf" ns :: In "len" ns :: In "tmp" ns :: In start ns :: In len ns
-    :: NoDup ("buf" :: "len" :: "tmp" :: start :: len :: nil)
-    :: (res >= 4)%nat
-    :: "sys"!"printInt" ~~ im ~~> printIntS
+    Fixpoint OutList (xms : list xml) : chunk :=
+      match xms with
+        | nil => Skip
+        | xm :: xms' => (Out' xm;; OutList xms')
+      end%SP.
+  End OutList.
+
+  Fixpoint Out' (xm : xml) : chunk :=
+    match xm with
+      | Cdata data => StringWrite "obuf" "olen" "opos" "overflowed" data
+        invPre (fun a V _ => invPost a V)
+      | Tag tag inner =>
+        (StringWrite "obuf" "olen" "opos" "overflowed" ("<" ++ tag ++ ">")
+          invPre (fun a V _ => invPost a V);;
+         OutList Out' inner;;
+         StringWrite "obuf" "olen" "opos" "overflowed" ("</" ++ tag ++ ">")
+          invPre (fun a V _ => invPost a V))
+    end%SP.
+
+  Notation OutVcs xm := (fun im ns res =>
+    (~In "rp" ns) :: In "obuf" ns :: In "olen" ns :: In "opos" ns :: In "overflowed" ns
+    :: (forall a V V', (forall x, x <> "overflowed" -> x <> "opos" -> sel V x = sel V' x)
+      -> invPre a V ===> invPre a V')
+    :: (forall a V V', (forall x, x <> "overflowed" -> x <> "opos" -> sel V x = sel V' x)
+      -> invPost a V = invPost a V')
+    :: wf xm
     :: nil).
 
   Opaque mult.
 
-  Lemma inv_sel : forall V, inv (sel V) = inv V.
+  Lemma invPre_sel : forall a V, invPre a (sel V) = invPre a V.
     auto.
   Qed.
 
-  Lemma wplus_wminus : forall u v : W,
-    u ^+ v ^- v = u.
-    intros; words.
-  Qed.
-
-  Hint Rewrite wplus_wminus : sepFormula.
-
-  Lemma mult4_S : forall n,
-    4 * S n = S (S (S (S (4 * n)))).
-    simpl; intros; omega.
+  Lemma invPost_sel : forall a V, invPost a (sel V) = invPost a V.
+    auto.
   Qed.
 
   Ltac prep :=
@@ -62,11 +127,21 @@ Section Out.
 
   Ltac simp :=
     repeat match goal with
-             | [ H : context[inv (sel ?V)] |- _ ] => rewrite (inv_sel V) in H
-             | [ |- context[inv (sel ?V)] ] => rewrite (inv_sel V)
-           end; repeat rewrite <- mult4_S in *; reger.
+             | [ H : context[invPre ?a (sel ?V)] |- _ ] => rewrite (invPre_sel a V) in H
+             | [ |- context[invPre ?a (sel ?V)] ] => rewrite (invPre_sel a V)
+             | [ H : context[invPost ?a (sel ?V)] |- _ ] => rewrite (invPost_sel a V) in H
+             | [ |- context[invPost ?a (sel ?V)] ] => rewrite (invPost_sel a V)
+           end; reger.
 
-  Ltac prepl := post; unfold lvalIn, regInL, immInR in *; prep_locals; simp.
+  Ltac prepl := post; unfold lvalIn, regInL, immInR in *;
+    repeat match goal with
+             | [ H : ForallR _ _ |- _ ] => clear H
+             | [ H : List.Forall _ _ |- _ ] => clear H
+             | [ H : importsGlobal _ |- _ ] =>
+               repeat match goal with
+                        | [ H' : context[H] |- _ ] => clear H'
+                      end; clear H
+           end; prep_locals; simp.
 
   Ltac my_descend :=
     repeat match goal with
@@ -78,21 +153,91 @@ Section Out.
   Ltac invoke1 :=
     match goal with
       | [ H : interp _ _, H' : _ |- _ ] => apply H' in H; clear H'
+      | [ |- vcs (_ :: _) ] => wrap0; try discriminate
+      | [ H : _ |- vcs _ ] => apply vcs_app_fwd || apply H
     end; post.
 
   Ltac t := post; repeat invoke1; prep; propxFo;
     repeat invoke1; prepl;
       evaluate auto_ext; my_descend; (repeat (step auto_ext; my_descend); auto).
 
-  Definition Out : chunk.
-    refine (WrapC (Call "sys"!"printInt"(start)
-                   [invar];;
-                   Call "sys"!"printInt"(len)
-                   [invar])%SP
+  Section Out_correct.
+    Variables (im : LabelMap.t assert) (mn : string) (H : importsGlobal im) (ns : list string) (res : nat).
+
+    Hypothesis Hrp : ~In "rp" ns.
+    Hypothesis Hobuf : In "obuf" ns.
+    Hypothesis Holen : In "olen" ns.
+    Hypothesis Hopos : In "opos" ns.
+    Hypothesis Hoverflowed : In "overflowed" ns.
+    Hypothesis HinvPre : forall a V V', (forall x, x <> "overflowed" -> x <> "opos" -> sel V x = sel V' x)
+      -> invPre a V ===> invPre a V'.
+    Hypothesis HinvPost : forall a V V', (forall x, x <> "overflowed" -> x <> "opos" -> sel V x = sel V' x)
+      -> invPost a V = invPost a V'.
+
+    Ltac split_IH :=
+      match goal with
+        | [ IH : forall pre : settings * state -> _, _ |- _ ] =>
+          (generalize (fun a b => proj1 (IH a b));
+            generalize (fun a b => proj2 (IH a b)))
+          || (generalize (fun a b c => proj1 (IH a b c));
+            generalize (fun a b c => proj2 (IH a b c))); clear IH; intros
+      end.
+
+    Lemma OutList_correct : forall xms,
+      List.Forall
+      (fun xm => forall pre, wf xm
+        -> (forall specs st, interp specs (pre st)
+          -> interp specs (invar true (fun x => x) ns res st))
+        -> (forall specs st,
+          interp specs (Postcondition (toCmd (Out' xm) mn H ns res pre) st)
+          -> interp specs (invar true (fun x => x) ns res st))
+        /\ vcs (VerifCond (toCmd (Out' xm) mn H ns res pre))) xms
+      -> ForallR wf xms
+      -> forall pre,
+        (forall specs st, interp specs (pre st)
+          -> interp specs (invar true (fun x => x) ns res st))
+        -> (forall specs st, interp specs (Postcondition (toCmd (OutList Out' xms) mn H ns res pre) st)
+            -> interp specs (invar true (fun x => x) ns res st))
+          /\ vcs (VerifCond (toCmd (OutList Out' xms) mn H ns res pre)).
+      induction 1; post; intuition; repeat split_IH; t.
+    Qed.
+
+    Hint Constructors unit.
+
+    Lemma length_append : forall s1 s2, String.length (s1 ++ s2) = String.length s1 + String.length s2.
+      induction s1; simpl; intuition.
+    Qed.
+
+    Hint Rewrite length_append : sepFormula.
+
+    Hint Extern 1 (goodSize _) => eapply goodSize_weaken; [ eassumption | omega ].
+
+    Lemma Out_correct : forall xm pre,
+      wf xm
+      -> (forall specs st, interp specs (pre st)
+        -> interp specs (invar true (fun x => x) ns res st))
+      -> (forall specs st, interp specs (Postcondition (toCmd (Out' xm) mn H ns res pre) st)
+        -> interp specs (invar true (fun x => x) ns res st))
+      /\ vcs (VerifCond (toCmd (Out' xm) mn H ns res pre)).
+      induction xm using xml_ind'; (post; try match goal with
+                                                | [ |- vcs (_ :: _) ] => wrap0; try discriminate
+                                              end;
+      solve [ t | match goal with
+                    | [ H : List.Forall _ _ |- _ ] =>
+                      eapply OutList_correct in H; [ destruct H; eauto | auto | ]
+                  end; t ]).
+    Qed.
+  End Out_correct.
+
+  Definition Out (xm : xml) : chunk.
+    refine (WrapC (Out' xm)
       invar
       invar
-      OutVcs
-      _ _); abstract (wrap0; t).
+      (OutVcs xm)
+      _ _); abstract (wrap0;
+        match goal with
+          | [ H : wf _ |- _ ] => eapply Out_correct in H; eauto
+        end; t).
   Defined.
 
 End Out.
